floyd/entailer.v
@@ -925,3 +925,18 @@ match goal with
   H1: Znth ?x (?s ++ [Byte.zero]) = Byte.zero |- _ =>
   is_var x; assert  (x = Zlength s) by cstring; subst x
 end.
+
+Lemma ptrofs_of_int64_int64_repr:
+  Archi.ptr64=true ->
+  forall i, Ptrofs.of_int64 (Int64.repr i) = Ptrofs.repr i.
+Proof.
+intros.
+unfold Ptrofs.of_int64.
+apply efield_lemmas.Ptrofs_repr_Int64_unsigned_special; auto.
+Qed.
+
+(* new experiment *)
+(* #[export] Hint Rewrite ptrofs_of_int64_int64_repr using reflexivity : norm rep_lia. *)
+#[export] Hint Rewrite Ptrofs.signed_repr using rep_lia : norm.
+#[export] Hint Rewrite Ptrofs.unsigned_repr using rep_lia : norm. 
+(* end new experiment *)
